Integrate new prelude with translator.
This takes up the work Shaz did on the new memory and array encoding and integrates it with the translator. The prelude has also been tweaked a bit:

- Sectioninzing, rearranging, and documenting for better readability.
- Adding helpers to abstract from actual memory model for the translated code. This should allows us for now to easier experiment with the encoding.
- Fixing some type check errors.

Nothing has been tested yet with real verification, but with this change we should be ready to do so.

Closes: #2094
Approved by: sblackshear,cbarrettfb

language/move-prover/bytecode-to-boogie/src/driver.rs
@@ -18,7 +18,7 @@ use std::process::Command;
 use vm::file_format::FunctionDefinitionIndex;
 
 /// Content of the default prelude.
-const DEFAULT_PRELUDE: &[u8] = include_bytes!("bytecode_instrs.bpl");
+const DEFAULT_PRELUDE: &[u8] = include_bytes!("prelude.bpl");
 
 /// Represents the driver for translation. This is the top-level object which owns
 /// all data during the steps of translation. Phases of the translation refer back to it.
