language/move-prover/bytecode-to-boogie/tests/goldenfiles/test-control-flow.bpl
@@ -4,62 +4,10 @@
 
 
 
-// ** stratified functions
-
-procedure {:inline 1} ReadValue0(p: Path, i: int, v: Value) returns (v': Value)
-{
-    var e: Edge;
-    if (i == size#Path(p)) {
-        v' := v;
-    } else {
-        assert false;
-    }
-}
-
-procedure {:inline 1} ReadValueMax(p: Path, i: int, v: Value) returns (v': Value)
-{
-    var e: Edge;
-    if (i == size#Path(p)) {
-        v' := v;
-    } else {
-        e := p#Path(p)[i];
-        if (is#Struct(v)) { v' := smap(v)[f#Field(e)]; }
-        if (is#Vector(v)) { v' := vmap(v)[i#Index(e)]; }
-        call v' := ReadValue0(p, i+1, v');
-    }
-}
-
-procedure {:inline 1} UpdateValue0(p: Path, i: int, v: Value, new_v: Value) returns (v': Value)
-{
-    var e: Edge;
-    if (i == size#Path(p)) {
-        v' := new_v;
-    } else {
-        assert false;
-    }
-}
-
-procedure {:inline 1} UpdateValueMax(p: Path, i: int, v: Value, new_v: Value) returns (v': Value)
-{
-    var e: Edge;
-    if (i == size#Path(p)) {
-        v' := new_v;
-    } else {
-        e := p#Path(p)[i];
-        if (is#Struct(v)) { v' := smap(v)[f#Field(e)]; }
-        if (is#Vector(v)) { v' := vmap(v)[i#Index(e)]; }
-        call v' := UpdateValue0(p, i+1, v', new_v);
-        if (is#Struct(v)) { v' := mk_struct(smap(v)[f#Field(e) := v'], slen(v));}
-        if (is#Vector(v)) { v' := mk_vector(vmap(v)[i#Index(e) := v'], vlen(v));}
-    }
-}
-
-
-
 // ** functions of module TestControlFlow
 
 procedure {:inline 1} TestControlFlow_branch_once (arg0: Value) returns (ret0: Value)
-requires ExistsTxnSenderAccount();
+requires ExistsTxnSenderAccount(m, txn);
 {
     // declare local variables
     var t0: Value; // BooleanType()
@@ -74,36 +22,36 @@ requires ExistsTxnSenderAccount();
     assume !abort_flag;
 
     // assume arguments are of correct types
-    assume has_type(BooleanType(), arg0);
+    assume is#Boolean(arg0);
 
-    old_size := m_size;
-    m_size := m_size + 6;
-    m := Memory(domain#Memory(m)[0+old_size := true], contents#Memory(m)[0+old_size :=  arg0]);
+    old_size := local_counter;
+    local_counter := local_counter + 6;
+    m := UpdateLocal(m, old_size + 0, arg0);
 
     // bytecode translation starts here
-    call tmp := CopyOrMoveValue(contents#Memory(m)[old_size+0]);
-    m := Memory(domain#Memory(m)[1+old_size := true], contents#Memory(m)[1+old_size := tmp]);
+    call tmp := CopyOrMoveValue(GetLocal(m, old_size + 0));
+    m := UpdateLocal(m, old_size + 1, tmp);
 
-    tmp := contents#Memory(m)[old_size + 1];
+    tmp := GetLocal(m, old_size + 1);
     if (!b#Boolean(tmp)) { goto Label_6; }
 
     call tmp := LdConst(1);
-    m := Memory(domain#Memory(m)[2+old_size := true], contents#Memory(m)[2+old_size := tmp]);
+    m := UpdateLocal(m, old_size + 2, tmp);
 
     call tmp := LdConst(2);
-    m := Memory(domain#Memory(m)[3+old_size := true], contents#Memory(m)[3+old_size := tmp]);
+    m := UpdateLocal(m, old_size + 3, tmp);
 
-    call tmp := Add(contents#Memory(m)[old_size+2], contents#Memory(m)[old_size+3]);
-    m := Memory(domain#Memory(m)[4+old_size := true], contents#Memory(m)[4+old_size := tmp]);
+    call tmp := Add(GetLocal(m, old_size + 2), GetLocal(m, old_size + 3));
+    m := UpdateLocal(m, old_size + 4, tmp);
 
-    ret0 := contents#Memory(m)[old_size+4];
+    ret0 := GetLocal(m, old_size + 4);
     return;
 
 Label_6:
     call tmp := LdConst(0);
-    m := Memory(domain#Memory(m)[5+old_size := true], contents#Memory(m)[5+old_size := tmp]);
+    m := UpdateLocal(m, old_size + 5, tmp);
 
-    ret0 := contents#Memory(m)[old_size+5];
+    ret0 := GetLocal(m, old_size + 5);
     return;
 
 }
