language/move-prover/bytecode-to-boogie/tests/goldenfiles/test-generics.bpl
@@ -6,120 +6,40 @@ const unique TestGenerics_R: TypeName;
 const TestGenerics_R_v: FieldName;
 axiom TestGenerics_R_v == 0;
 function TestGenerics_R_type_value(): TypeValue {
-    StructType(TestGenerics_R, TypeValueArray(DefaultTypeMap[0 := Vector_T_type_value(IntegerType())], 1))
+    StructType(TestGenerics_R, ExtendTypeValueArray(EmptyTypeValueArray, Vector_T_type_value(IntegerType())))
 }
 
 procedure {:inline 1} Pack_TestGenerics_R(v0: Value) returns (v: Value)
 {
-    assume has_type(Vector_T_type_value(IntegerType()), v0);
-    v := Struct(ValueArray(DefaultIntMap[TestGenerics_R_v := v0], 1));
-    assume has_type(TestGenerics_R_type_value(), v);
+    assume is#Vector(v0);
+    v := Vector(ExtendValueArray(EmptyValueArray, v0));
+
 }
 
 procedure {:inline 1} Unpack_TestGenerics_R(v: Value) returns (v0: Value)
 {
-    assert is#Struct(v);
-    v0 := smap(v)[TestGenerics_R_v];
+    assume is#Vector(v);
+    v0 := SelectField(v, TestGenerics_R_v);
 }
 
 const unique TestGenerics_T: TypeName;
 const TestGenerics_T_v: FieldName;
 axiom TestGenerics_T_v == 0;
 function TestGenerics_T_type_value(tv0: TypeValue): TypeValue {
-    StructType(TestGenerics_T, TypeValueArray(DefaultTypeMap[0 := Vector_T_type_value(tv0)], 1))
+    StructType(TestGenerics_T, ExtendTypeValueArray(EmptyTypeValueArray, Vector_T_type_value(tv0)))
 }
 
 procedure {:inline 1} Pack_TestGenerics_T(tv0: TypeValue, v0: Value) returns (v: Value)
 {
-    assume has_type(Vector_T_type_value(tv0), v0);
-    v := Struct(ValueArray(DefaultIntMap[TestGenerics_T_v := v0], 1));
-    assume has_type(TestGenerics_T_type_value(tv0), v);
+    assume is#Vector(v0);
+    v := Vector(ExtendValueArray(EmptyValueArray, v0));
+
 }
 
 procedure {:inline 1} Unpack_TestGenerics_T(v: Value) returns (v0: Value)
 {
-    assert is#Struct(v);
-    v0 := smap(v)[TestGenerics_T_v];
-}
-
-
-
-// ** stratified functions
-
-procedure {:inline 1} ReadValue0(p: Path, i: int, v: Value) returns (v': Value)
-{
-    var e: Edge;
-    if (i == size#Path(p)) {
-        v' := v;
-    } else {
-        assert false;
-    }
-}
-
-procedure {:inline 1} ReadValue1(p: Path, i: int, v: Value) returns (v': Value)
-{
-    var e: Edge;
-    if (i == size#Path(p)) {
-        v' := v;
-    } else {
-        e := p#Path(p)[i];
-        if (is#Struct(v)) { v' := smap(v)[f#Field(e)]; }
-        if (is#Vector(v)) { v' := vmap(v)[i#Index(e)]; }
-        call v' := ReadValue0(p, i+1, v');
-    }
-}
-
-procedure {:inline 1} ReadValueMax(p: Path, i: int, v: Value) returns (v': Value)
-{
-    var e: Edge;
-    if (i == size#Path(p)) {
-        v' := v;
-    } else {
-        e := p#Path(p)[i];
-        if (is#Struct(v)) { v' := smap(v)[f#Field(e)]; }
-        if (is#Vector(v)) { v' := vmap(v)[i#Index(e)]; }
-        call v' := ReadValue1(p, i+1, v');
-    }
-}
-
-procedure {:inline 1} UpdateValue0(p: Path, i: int, v: Value, new_v: Value) returns (v': Value)
-{
-    var e: Edge;
-    if (i == size#Path(p)) {
-        v' := new_v;
-    } else {
-        assert false;
-    }
-}
-
-procedure {:inline 1} UpdateValue1(p: Path, i: int, v: Value, new_v: Value) returns (v': Value)
-{
-    var e: Edge;
-    if (i == size#Path(p)) {
-        v' := new_v;
-    } else {
-        e := p#Path(p)[i];
-        if (is#Struct(v)) { v' := smap(v)[f#Field(e)]; }
-        if (is#Vector(v)) { v' := vmap(v)[i#Index(e)]; }
-        call v' := UpdateValue0(p, i+1, v', new_v);
-        if (is#Struct(v)) { v' := mk_struct(smap(v)[f#Field(e) := v'], slen(v));}
-        if (is#Vector(v)) { v' := mk_vector(vmap(v)[i#Index(e) := v'], vlen(v));}
-    }
-}
-
-procedure {:inline 1} UpdateValueMax(p: Path, i: int, v: Value, new_v: Value) returns (v': Value)
-{
-    var e: Edge;
-    if (i == size#Path(p)) {
-        v' := new_v;
-    } else {
-        e := p#Path(p)[i];
-        if (is#Struct(v)) { v' := smap(v)[f#Field(e)]; }
-        if (is#Vector(v)) { v' := vmap(v)[i#Index(e)]; }
-        call v' := UpdateValue1(p, i+1, v', new_v);
-        if (is#Struct(v)) { v' := mk_struct(smap(v)[f#Field(e) := v'], slen(v));}
-        if (is#Vector(v)) { v' := mk_vector(vmap(v)[i#Index(e) := v'], vlen(v));}
-    }
+    assume is#Vector(v);
+    v0 := SelectField(v, TestGenerics_T_v);
 }
 
 
@@ -127,7 +47,7 @@ procedure {:inline 1} UpdateValueMax(p: Path, i: int, v: Value, new_v: Value) re
 // ** functions of module TestGenerics
 
 procedure {:inline 1} TestGenerics_move2 (arg0: Value, arg1: Value) returns ()
-requires ExistsTxnSenderAccount();
+requires ExistsTxnSenderAccount(m, txn);
 {
     // declare local variables
     var t0: Value; // IntegerType()
@@ -148,52 +68,52 @@ requires ExistsTxnSenderAccount();
     assume !abort_flag;
 
     // assume arguments are of correct types
-    assume has_type(IntegerType(), arg0);
-    assume has_type(IntegerType(), arg1);
+    assume is#Integer(arg0);
+    assume is#Integer(arg1);
 
-    old_size := m_size;
-    m_size := m_size + 12;
-    m := Memory(domain#Memory(m)[0+old_size := true], contents#Memory(m)[0+old_size :=  arg0]);
-    m := Memory(domain#Memory(m)[1+old_size := true], contents#Memory(m)[1+old_size :=  arg1]);
+    old_size := local_counter;
+    local_counter := local_counter + 12;
+    m := UpdateLocal(m, old_size + 0, arg0);
+    m := UpdateLocal(m, old_size + 1, arg1);
 
     // bytecode translation starts here
     call t4 := Vector_empty(IntegerType());
-    assume has_type(Vector_T_type_value(IntegerType()), t4);
+    assume is#Vector(t4);
 
-    m := Memory(domain#Memory(m)[old_size+4 := true], contents#Memory(m)[old_size+4 := t4]);
+    m := UpdateLocal(m, old_size + 4, t4);
 
-    call tmp := CopyOrMoveValue(contents#Memory(m)[old_size+4]);
-    m := Memory(domain#Memory(m)[2+old_size := true], contents#Memory(m)[2+old_size := tmp]);
+    call tmp := CopyOrMoveValue(GetLocal(m, old_size + 4));
+    m := UpdateLocal(m, old_size + 2, tmp);
 
     call t5 := BorrowLoc(old_size+2);
 
-    call tmp := CopyOrMoveValue(contents#Memory(m)[old_size+0]);
-    m := Memory(domain#Memory(m)[6+old_size := true], contents#Memory(m)[6+old_size := tmp]);
+    call tmp := CopyOrMoveValue(GetLocal(m, old_size + 0));
+    m := UpdateLocal(m, old_size + 6, tmp);
 
-    call Vector_push_back(IntegerType(), t5, contents#Memory(m)[old_size+6]);
+    call Vector_push_back(IntegerType(), t5, GetLocal(m, old_size + 6));
 
     call t7 := BorrowLoc(old_size+2);
 
-    call tmp := CopyOrMoveValue(contents#Memory(m)[old_size+1]);
-    m := Memory(domain#Memory(m)[8+old_size := true], contents#Memory(m)[8+old_size := tmp]);
+    call tmp := CopyOrMoveValue(GetLocal(m, old_size + 1));
+    m := UpdateLocal(m, old_size + 8, tmp);
 
-    call Vector_push_back(IntegerType(), t7, contents#Memory(m)[old_size+8]);
+    call Vector_push_back(IntegerType(), t7, GetLocal(m, old_size + 8));
 
-    call tmp := CopyOrMoveValue(contents#Memory(m)[old_size+2]);
-    m := Memory(domain#Memory(m)[9+old_size := true], contents#Memory(m)[9+old_size := tmp]);
+    call tmp := CopyOrMoveValue(GetLocal(m, old_size + 2));
+    m := UpdateLocal(m, old_size + 9, tmp);
 
-    assume has_type(Vector_T_type_value(IntegerType()), contents#Memory(m)[old_size+9]);
+    assume is#Vector(GetLocal(m, old_size + 9));
 
-    call tmp := Pack_TestGenerics_R(contents#Memory(m)[old_size+9]);
-    m := Memory(domain#Memory(m)[10+old_size := true], contents#Memory(m)[10+old_size := tmp]);
+    call tmp := Pack_TestGenerics_R(GetLocal(m, old_size + 9));
+    m := UpdateLocal(m, old_size + 10, tmp);
 
-    call tmp := CopyOrMoveValue(contents#Memory(m)[old_size+10]);
-    m := Memory(domain#Memory(m)[3+old_size := true], contents#Memory(m)[3+old_size := tmp]);
+    call tmp := CopyOrMoveValue(GetLocal(m, old_size + 10));
+    m := UpdateLocal(m, old_size + 3, tmp);
 
-    call tmp := CopyOrMoveValue(contents#Memory(m)[old_size+3]);
-    m := Memory(domain#Memory(m)[11+old_size := true], contents#Memory(m)[11+old_size := tmp]);
+    call tmp := CopyOrMoveValue(GetLocal(m, old_size + 3));
+    m := UpdateLocal(m, old_size + 11, tmp);
 
-    call MoveToSender(TestGenerics_R_type_value(), contents#Memory(m)[old_size+11]);
+    call MoveToSender(TestGenerics_R_type_value(), GetLocal(m, old_size + 11));
 
     return;
 
@@ -205,7 +125,7 @@ procedure TestGenerics_move2_verify (arg0: Value, arg1: Value) returns ()
 }
 
 procedure {:inline 1} TestGenerics_create (tv0: TypeValue, arg0: Value) returns (ret0: Value)
-requires ExistsTxnSenderAccount();
+requires ExistsTxnSenderAccount(m, txn);
 {
     // declare local variables
     var t0: Value; // tv0
@@ -221,37 +141,36 @@ requires ExistsTxnSenderAccount();
     assume !abort_flag;
 
     // assume arguments are of correct types
-    assume has_type(tv0, arg0);
 
-    old_size := m_size;
-    m_size := m_size + 7;
-    m := Memory(domain#Memory(m)[0+old_size := true], contents#Memory(m)[0+old_size :=  arg0]);
+    old_size := local_counter;
+    local_counter := local_counter + 7;
+    m := UpdateLocal(m, old_size + 0, arg0);
 
     // bytecode translation starts here
     call t2 := Vector_empty(tv0);
-    assume has_type(Vector_T_type_value(tv0), t2);
+    assume is#Vector(t2);
 
-    m := Memory(domain#Memory(m)[old_size+2 := true], contents#Memory(m)[old_size+2 := t2]);
+    m := UpdateLocal(m, old_size + 2, t2);
 
-    call tmp := CopyOrMoveValue(contents#Memory(m)[old_size+2]);
-    m := Memory(domain#Memory(m)[1+old_size := true], contents#Memory(m)[1+old_size := tmp]);
+    call tmp := CopyOrMoveValue(GetLocal(m, old_size + 2));
+    m := UpdateLocal(m, old_size + 1, tmp);
 
     call t3 := BorrowLoc(old_size+1);
 
-    call tmp := CopyOrMoveValue(contents#Memory(m)[old_size+0]);
-    m := Memory(domain#Memory(m)[4+old_size := true], contents#Memory(m)[4+old_size := tmp]);
+    call tmp := CopyOrMoveValue(GetLocal(m, old_size + 0));
+    m := UpdateLocal(m, old_size + 4, tmp);
 
-    call Vector_push_back(tv0, t3, contents#Memory(m)[old_size+4]);
+    call Vector_push_back(tv0, t3, GetLocal(m, old_size + 4));
 
-    call tmp := CopyOrMoveValue(contents#Memory(m)[old_size+1]);
-    m := Memory(domain#Memory(m)[5+old_size := true], contents#Memory(m)[5+old_size := tmp]);
+    call tmp := CopyOrMoveValue(GetLocal(m, old_size + 1));
+    m := UpdateLocal(m, old_size + 5, tmp);
 
-    assume has_type(Vector_T_type_value(tv0), contents#Memory(m)[old_size+5]);
+    assume is#Vector(GetLocal(m, old_size + 5));
 
-    call tmp := Pack_TestGenerics_T(tv0, contents#Memory(m)[old_size+5]);
-    m := Memory(domain#Memory(m)[6+old_size := true], contents#Memory(m)[6+old_size := tmp]);
+    call tmp := Pack_TestGenerics_T(tv0, GetLocal(m, old_size + 5));
+    m := UpdateLocal(m, old_size + 6, tmp);
 
-    ret0 := contents#Memory(m)[old_size+6];
+    ret0 := GetLocal(m, old_size + 6);
     return;
 
 }
@@ -262,7 +181,7 @@ procedure TestGenerics_create_verify (tv0: TypeValue, arg0: Value) returns (ret0
 }
 
 procedure {:inline 1} TestGenerics_overcomplicated_equals (tv0: TypeValue, arg0: Value, arg1: Value) returns (ret0: Value)
-requires ExistsTxnSenderAccount();
+requires ExistsTxnSenderAccount(m, txn);
 {
     // declare local variables
     var t0: Value; // tv0
@@ -284,53 +203,51 @@ requires ExistsTxnSenderAccount();
     assume !abort_flag;
 
     // assume arguments are of correct types
-    assume has_type(tv0, arg0);
-    assume has_type(tv0, arg1);
 
-    old_size := m_size;
-    m_size := m_size + 13;
-    m := Memory(domain#Memory(m)[0+old_size := true], contents#Memory(m)[0+old_size :=  arg0]);
-    m := Memory(domain#Memory(m)[1+old_size := true], contents#Memory(m)[1+old_size :=  arg1]);
+    old_size := local_counter;
+    local_counter := local_counter + 13;
+    m := UpdateLocal(m, old_size + 0, arg0);
+    m := UpdateLocal(m, old_size + 1, arg1);
 
     // bytecode translation starts here
-    call tmp := CopyOrMoveValue(contents#Memory(m)[old_size+0]);
-    m := Memory(domain#Memory(m)[5+old_size := true], contents#Memory(m)[5+old_size := tmp]);
+    call tmp := CopyOrMoveValue(GetLocal(m, old_size + 0));
+    m := UpdateLocal(m, old_size + 5, tmp);
 
-    call t6 := TestGenerics_create(tv0, contents#Memory(m)[old_size+5]);
-    assume has_type(TestGenerics_T_type_value(tv0), t6);
+    call t6 := TestGenerics_create(tv0, GetLocal(m, old_size + 5));
+    assume is#Vector(t6);
 
-    m := Memory(domain#Memory(m)[old_size+6 := true], contents#Memory(m)[old_size+6 := t6]);
+    m := UpdateLocal(m, old_size + 6, t6);
 
-    call tmp := CopyOrMoveValue(contents#Memory(m)[old_size+6]);
-    m := Memory(domain#Memory(m)[3+old_size := true], contents#Memory(m)[3+old_size := tmp]);
+    call tmp := CopyOrMoveValue(GetLocal(m, old_size + 6));
+    m := UpdateLocal(m, old_size + 3, tmp);
 
-    call tmp := CopyOrMoveValue(contents#Memory(m)[old_size+1]);
-    m := Memory(domain#Memory(m)[7+old_size := true], contents#Memory(m)[7+old_size := tmp]);
+    call tmp := CopyOrMoveValue(GetLocal(m, old_size + 1));
+    m := UpdateLocal(m, old_size + 7, tmp);
 
-    call t8 := TestGenerics_create(tv0, contents#Memory(m)[old_size+7]);
-    assume has_type(TestGenerics_T_type_value(tv0), t8);
+    call t8 := TestGenerics_create(tv0, GetLocal(m, old_size + 7));
+    assume is#Vector(t8);
 
-    m := Memory(domain#Memory(m)[old_size+8 := true], contents#Memory(m)[old_size+8 := t8]);
+    m := UpdateLocal(m, old_size + 8, t8);
 
-    call tmp := CopyOrMoveValue(contents#Memory(m)[old_size+8]);
-    m := Memory(domain#Memory(m)[4+old_size := true], contents#Memory(m)[4+old_size := tmp]);
+    call tmp := CopyOrMoveValue(GetLocal(m, old_size + 8));
+    m := UpdateLocal(m, old_size + 4, tmp);
 
-    call tmp := CopyOrMoveValue(contents#Memory(m)[old_size+3]);
-    m := Memory(domain#Memory(m)[9+old_size := true], contents#Memory(m)[9+old_size := tmp]);
+    call tmp := CopyOrMoveValue(GetLocal(m, old_size + 3));
+    m := UpdateLocal(m, old_size + 9, tmp);
 
-    call tmp := CopyOrMoveValue(contents#Memory(m)[old_size+4]);
-    m := Memory(domain#Memory(m)[10+old_size := true], contents#Memory(m)[10+old_size := tmp]);
+    call tmp := CopyOrMoveValue(GetLocal(m, old_size + 4));
+    m := UpdateLocal(m, old_size + 10, tmp);
 
-    tmp := Boolean(is_equal(TestGenerics_T_type_value(tv0), contents#Memory(m)[old_size+9], contents#Memory(m)[old_size+10]));
-    m := Memory(domain#Memory(m)[11+old_size := true], contents#Memory(m)[11+old_size := tmp]);
+    tmp := Boolean(IsEqual(GetLocal(m, old_size + 9), GetLocal(m, old_size + 10)));
+    m := UpdateLocal(m, old_size + 11, tmp);
 
-    call tmp := CopyOrMoveValue(contents#Memory(m)[old_size+11]);
-    m := Memory(domain#Memory(m)[2+old_size := true], contents#Memory(m)[2+old_size := tmp]);
+    call tmp := CopyOrMoveValue(GetLocal(m, old_size + 11));
+    m := UpdateLocal(m, old_size + 2, tmp);
 
-    call tmp := CopyOrMoveValue(contents#Memory(m)[old_size+2]);
-    m := Memory(domain#Memory(m)[12+old_size := true], contents#Memory(m)[12+old_size := tmp]);
+    call tmp := CopyOrMoveValue(GetLocal(m, old_size + 2));
+    m := UpdateLocal(m, old_size + 12, tmp);
 
-    ret0 := contents#Memory(m)[old_size+12];
+    ret0 := GetLocal(m, old_size + 12);
     return;
 
 }
@@ -341,7 +258,7 @@ procedure TestGenerics_overcomplicated_equals_verify (tv0: TypeValue, arg0: Valu
 }
 
 procedure {:inline 1} TestGenerics_test () returns (ret0: Value)
-requires ExistsTxnSenderAccount();
+requires ExistsTxnSenderAccount(m, txn);
 {
     // declare local variables
     var t0: Value; // BooleanType()
@@ -356,28 +273,28 @@ requires ExistsTxnSenderAccount();
 
     // assume arguments are of correct types
 
-    old_size := m_size;
-    m_size := m_size + 5;
+    old_size := local_counter;
+    local_counter := local_counter + 5;
 
     // bytecode translation starts here
     call tmp := LdConst(1);
-    m := Memory(domain#Memory(m)[1+old_size := true], contents#Memory(m)[1+old_size := tmp]);
+    m := UpdateLocal(m, old_size + 1, tmp);
 
     call tmp := LdConst(1);
-    m := Memory(domain#Memory(m)[2+old_size := true], contents#Memory(m)[2+old_size := tmp]);
+    m := UpdateLocal(m, old_size + 2, tmp);
 
-    call t3 := TestGenerics_overcomplicated_equals(IntegerType(), contents#Memory(m)[old_size+1], contents#Memory(m)[old_size+2]);
-    assume has_type(BooleanType(), t3);
+    call t3 := TestGenerics_overcomplicated_equals(IntegerType(), GetLocal(m, old_size + 1), GetLocal(m, old_size + 2));
+    assume is#Boolean(t3);
 
-    m := Memory(domain#Memory(m)[old_size+3 := true], contents#Memory(m)[old_size+3 := t3]);
+    m := UpdateLocal(m, old_size + 3, t3);
 
-    call tmp := CopyOrMoveValue(contents#Memory(m)[old_size+3]);
-    m := Memory(domain#Memory(m)[0+old_size := true], contents#Memory(m)[0+old_size := tmp]);
+    call tmp := CopyOrMoveValue(GetLocal(m, old_size + 3));
+    m := UpdateLocal(m, old_size + 0, tmp);
 
-    call tmp := CopyOrMoveValue(contents#Memory(m)[old_size+0]);
-    m := Memory(domain#Memory(m)[4+old_size := true], contents#Memory(m)[4+old_size := tmp]);
+    call tmp := CopyOrMoveValue(GetLocal(m, old_size + 0));
+    m := UpdateLocal(m, old_size + 4, tmp);
 
-    ret0 := contents#Memory(m)[old_size+4];
+    ret0 := GetLocal(m, old_size + 4);
     return;
 
 }
