language/move-prover/bytecode-to-boogie/tests/goldenfiles/test-reference.bpl
@@ -6,100 +6,20 @@ const unique TestReference_T: TypeName;
 const TestReference_T_value: FieldName;
 axiom TestReference_T_value == 0;
 function TestReference_T_type_value(): TypeValue {
-    StructType(TestReference_T, TypeValueArray(DefaultTypeMap[0 := IntegerType()], 1))
+    StructType(TestReference_T, ExtendTypeValueArray(EmptyTypeValueArray, IntegerType()))
 }
 
 procedure {:inline 1} Pack_TestReference_T(v0: Value) returns (v: Value)
 {
-    assume has_type(IntegerType(), v0);
-    v := Struct(ValueArray(DefaultIntMap[TestReference_T_value := v0], 1));
-    assume has_type(TestReference_T_type_value(), v);
+    assume is#Integer(v0);
+    v := Vector(ExtendValueArray(EmptyValueArray, v0));
+
 }
 
 procedure {:inline 1} Unpack_TestReference_T(v: Value) returns (v0: Value)
 {
-    assert is#Struct(v);
-    v0 := smap(v)[TestReference_T_value];
-}
-
-
-
-// ** stratified functions
-
-procedure {:inline 1} ReadValue0(p: Path, i: int, v: Value) returns (v': Value)
-{
-    var e: Edge;
-    if (i == size#Path(p)) {
-        v' := v;
-    } else {
-        assert false;
-    }
-}
-
-procedure {:inline 1} ReadValue1(p: Path, i: int, v: Value) returns (v': Value)
-{
-    var e: Edge;
-    if (i == size#Path(p)) {
-        v' := v;
-    } else {
-        e := p#Path(p)[i];
-        if (is#Struct(v)) { v' := smap(v)[f#Field(e)]; }
-        if (is#Vector(v)) { v' := vmap(v)[i#Index(e)]; }
-        call v' := ReadValue0(p, i+1, v');
-    }
-}
-
-procedure {:inline 1} ReadValueMax(p: Path, i: int, v: Value) returns (v': Value)
-{
-    var e: Edge;
-    if (i == size#Path(p)) {
-        v' := v;
-    } else {
-        e := p#Path(p)[i];
-        if (is#Struct(v)) { v' := smap(v)[f#Field(e)]; }
-        if (is#Vector(v)) { v' := vmap(v)[i#Index(e)]; }
-        call v' := ReadValue1(p, i+1, v');
-    }
-}
-
-procedure {:inline 1} UpdateValue0(p: Path, i: int, v: Value, new_v: Value) returns (v': Value)
-{
-    var e: Edge;
-    if (i == size#Path(p)) {
-        v' := new_v;
-    } else {
-        assert false;
-    }
-}
-
-procedure {:inline 1} UpdateValue1(p: Path, i: int, v: Value, new_v: Value) returns (v': Value)
-{
-    var e: Edge;
-    if (i == size#Path(p)) {
-        v' := new_v;
-    } else {
-        e := p#Path(p)[i];
-        if (is#Struct(v)) { v' := smap(v)[f#Field(e)]; }
-        if (is#Vector(v)) { v' := vmap(v)[i#Index(e)]; }
-        call v' := UpdateValue0(p, i+1, v', new_v);
-        if (is#Struct(v)) { v' := mk_struct(smap(v)[f#Field(e) := v'], slen(v));}
-        if (is#Vector(v)) { v' := mk_vector(vmap(v)[i#Index(e) := v'], vlen(v));}
-    }
-}
-
-procedure {:inline 1} UpdateValueMax(p: Path, i: int, v: Value, new_v: Value) returns (v': Value)
-{
-    var e: Edge;
-    if (i == size#Path(p)) {
-        v' := new_v;
-    } else {
-        e := p#Path(p)[i];
-        if (is#Struct(v)) { v' := smap(v)[f#Field(e)]; }
-        if (is#Vector(v)) { v' := vmap(v)[i#Index(e)]; }
-        call v' := UpdateValue1(p, i+1, v', new_v);
-        if (is#Struct(v)) { v' := mk_struct(smap(v)[f#Field(e) := v'], slen(v));}
-        if (is#Vector(v)) { v' := mk_vector(vmap(v)[i#Index(e) := v'], vlen(v));}
-    }
+    assume is#Vector(v);
+    v0 := SelectField(v, TestReference_T_value);
 }
 
 
@@ -107,7 +27,7 @@ procedure {:inline 1} UpdateValueMax(p: Path, i: int, v: Value, new_v: Value) re
 // ** functions of module TestReference
 
 procedure {:inline 1} TestReference_mut_b (arg0: Reference) returns ()
-requires ExistsTxnSenderAccount();
+requires ExistsTxnSenderAccount(m, txn);
 {
     // declare local variables
     var t0: Reference; // ReferenceType(IntegerType())
@@ -120,17 +40,17 @@ requires ExistsTxnSenderAccount();
 
     // assume arguments are of correct types
 
-    old_size := m_size;
-    m_size := m_size + 3;
+    old_size := local_counter;
+    local_counter := local_counter + 3;
     t0 := arg0;
 
     // bytecode translation starts here
     call tmp := LdConst(10);
-    m := Memory(domain#Memory(m)[1+old_size := true], contents#Memory(m)[1+old_size := tmp]);
+    m := UpdateLocal(m, old_size + 1, tmp);
 
     call t2 := CopyOrMoveRef(t0);
 
-    call WriteRef(t2, contents#Memory(m)[old_size+1]);
+    call WriteRef(t2, GetLocal(m, old_size + 1));
 
     return;
 
@@ -142,7 +62,7 @@ procedure TestReference_mut_b_verify (arg0: Reference) returns ()
 }
 
 procedure {:inline 1} TestReference_mut_ref () returns ()
-requires ExistsTxnSenderAccount();
+requires ExistsTxnSenderAccount(m, txn);
 {
     // declare local variables
     var t0: Value; // IntegerType()
@@ -164,15 +84,15 @@ requires ExistsTxnSenderAccount();
 
     // assume arguments are of correct types
 
-    old_size := m_size;
-    m_size := m_size + 12;
+    old_size := local_counter;
+    local_counter := local_counter + 12;
 
     // bytecode translation starts here
     call tmp := LdConst(20);
-    m := Memory(domain#Memory(m)[2+old_size := true], contents#Memory(m)[2+old_size := tmp]);
+    m := UpdateLocal(m, old_size + 2, tmp);
 
-    call tmp := CopyOrMoveValue(contents#Memory(m)[old_size+2]);
-    m := Memory(domain#Memory(m)[0+old_size := true], contents#Memory(m)[0+old_size := tmp]);
+    call tmp := CopyOrMoveValue(GetLocal(m, old_size + 2));
+    m := UpdateLocal(m, old_size + 0, tmp);
 
     call t3 := BorrowLoc(old_size+0);
 
@@ -185,30 +105,30 @@ requires ExistsTxnSenderAccount();
     call t5 := CopyOrMoveRef(t1);
 
     call tmp := ReadRef(t5);
-    assume has_type(IntegerType(), tmp);
+    assume is#Integer(tmp);
 
-    m := Memory(domain#Memory(m)[6+old_size := true], contents#Memory(m)[6+old_size := tmp]);
+    m := UpdateLocal(m, old_size + 6, tmp);
 
-    call tmp := CopyOrMoveValue(contents#Memory(m)[old_size+6]);
-    m := Memory(domain#Memory(m)[0+old_size := true], contents#Memory(m)[0+old_size := tmp]);
+    call tmp := CopyOrMoveValue(GetLocal(m, old_size + 6));
+    m := UpdateLocal(m, old_size + 0, tmp);
 
-    call tmp := CopyOrMoveValue(contents#Memory(m)[old_size+0]);
-    m := Memory(domain#Memory(m)[7+old_size := true], contents#Memory(m)[7+old_size := tmp]);
+    call tmp := CopyOrMoveValue(GetLocal(m, old_size + 0));
+    m := UpdateLocal(m, old_size + 7, tmp);
 
     call tmp := LdConst(10);
-    m := Memory(domain#Memory(m)[8+old_size := true], contents#Memory(m)[8+old_size := tmp]);
+    m := UpdateLocal(m, old_size + 8, tmp);
 
-    tmp := Boolean(is_equal(IntegerType(), contents#Memory(m)[old_size+7], contents#Memory(m)[old_size+8]));
-    m := Memory(domain#Memory(m)[9+old_size := true], contents#Memory(m)[9+old_size := tmp]);
+    tmp := Boolean(IsEqual(GetLocal(m, old_size + 7), GetLocal(m, old_size + 8)));
+    m := UpdateLocal(m, old_size + 9, tmp);
 
-    call tmp := Not(contents#Memory(m)[old_size+9]);
-    m := Memory(domain#Memory(m)[10+old_size := true], contents#Memory(m)[10+old_size := tmp]);
+    call tmp := Not(GetLocal(m, old_size + 9));
+    m := UpdateLocal(m, old_size + 10, tmp);
 
-    tmp := contents#Memory(m)[old_size + 10];
+    tmp := GetLocal(m, old_size + 10);
     if (!b#Boolean(tmp)) { goto Label_16; }
 
     call tmp := LdConst(42);
-    m := Memory(domain#Memory(m)[11+old_size := true], contents#Memory(m)[11+old_size := tmp]);
+    m := UpdateLocal(m, old_size + 11, tmp);
 
     assert false;
 
